interp_binop with word

bedrock2/src/Basic_bopnames.v
@@ -1,3 +1,5 @@
+Require Import Coq.ZArith.BinInt.
+Require Import coqutil.Word.Interface.
 Require bedrock2.Syntax.
 Require bedrock2.BasicALU.
 
@@ -22,3 +24,25 @@ Instance make (p: parameters) : Syntax.parameters := {|
 
 Instance BasicALU{p: parameters}: BasicALU.operations :=
   BasicALU.Build_operations _ add sub mul and or xor sru slu srs lts ltu eq.
+
+Section WithWord.
+  Context {width : Z} {word : word width}.
+  Definition interp_binop (bop : bopname) : word -> word -> word :=
+    match bop with
+    | bopname.add => word.add
+    | bopname.sub => word.sub
+    | bopname.mul => word.mul
+    | bopname.and => word.and
+    | bopname.or => word.or
+    | bopname.xor => word.xor
+    | bopname.sru => word.sru
+    | bopname.slu => word.slu
+    | bopname.srs => word.srs
+    | bopname.lts => fun a b =>
+      if word.lts a b then word.of_Z 1 else word.of_Z 0
+    | bopname.ltu => fun a b =>
+      if word.ltu a b then word.of_Z 1 else word.of_Z 0
+    | bopname.eq => fun a b =>
+      if word.eqb a b then word.of_Z 1 else word.of_Z 0
+    end.
+End WithWord.
