bedrock2/src/BasicC64Semantics.v
@@ -3,31 +3,15 @@ Require Import bedrock2.Syntax bedrock2.BasicC64Syntax bedrock2.Semantics.
 Require bedrock2.String bedrock2.Map.SortedList bedrock2.Map.SortedListString.
 Require Import coqutil.Word.Interface.
 Require coqutil.Word.Naive.
+
 Instance parameters : parameters :=
-  let word := Word.Naive.word 64 (proj2 (Zlt_is_lt_bool 0 64) eq_refl) in
-  let byte := Word.Naive.word 8 (proj2 (Zlt_is_lt_bool 0 8) eq_refl) in
+  let word := Word.Naive.word 64 eq_refl in
+  let byte := Word.Naive.word 8 eq_refl in
   {|
   syntax := StringNamesSyntax.make BasicC64Syntax.StringNames_params;
-  Semantics.word := word;
-  interp_binop bop :=
-    match bop with
-    | bopname.add => word.add
-    | bopname.sub => word.sub
-    | bopname.mul => word.mul
-    | bopname.and => word.and
-    | bopname.or  => word.or
-    | bopname.xor => word.xor
-    | bopname.sru => word.sru
-    | bopname.slu => word.slu
-    | bopname.srs => word.srs
-    | bopname.ltu => fun a b => if word.ltu a b then word.of_Z 1 else word.of_Z 0
-    | bopname.lts => fun a b => if word.lts a b then word.of_Z 1 else word.of_Z 0
-    | bopname.eq => fun a b => if word.eqb a b then word.of_Z 1 else word.of_Z 0
-    end;
-  (* TODO: bedrock2.Byte, bedrock2.Word8 *)
-  Semantics.byte := byte;
   mem := SortedList.map (SortedList.parameters.Build_parameters word byte word.eqb word.ltu);
   locals := SortedListString.map _;
+  interp_binop := Basic_bopnames.interp_binop;
   funname_eqb := String.eqb;
 |}.
 Existing Instance Word.Naive.ok.
